Returns_legacy now uses eutt instead of eq_itree

ccs/EquivalenceDO.v
@@ -253,63 +253,23 @@ Section EquivSem.
   Qed.
 
   Inductive Returns_legacy {E} {A: Type} (a: A) : itree E A -> Prop :=
-  | Returns_legacyRet: forall t, t ≅ Ret a -> Returns_legacy a t
-  | Returns_legacyTau: forall t u, t ≅ Tau u -> Returns_legacy a u -> Returns_legacy a t
+  | Returns_legacyRet: forall t, t ≈ Ret a -> Returns_legacy a t
   | Returns_legacyVis: forall {X} (e: E X) (x: X) t k,
-      t ≅ Vis e k -> Returns_legacy a (k x) -> Returns_legacy a t.
+      t ≈ Vis e k -> Returns_legacy a (k x) -> Returns_legacy a t.
 
-  Global Instance eq_itree_returns_leg {E A } (hd: A) :
-    Proper (@eq_itree E A A eq ==> flip impl) (Returns_legacy hd).
+  Global Instance Returns_legacy_eqit {E A} b hd :
+    Proper (eqit eq b b ==> flip impl) (@Returns_legacy E A hd).
   Proof.
     do 4 red.
     intros * Eq Ret.
-    revert Eq.
+    revert b x Eq.
     induction Ret;
-      intros.
-    - constructor.
-      now rewrite Eq.
-    - apply Returns_legacyTau with u.
-      + now rewrite Eq.
-      + assumption.
-    - eapply Returns_legacyVis.
-      + rewrite Eq.
-        apply H.
-      + apply Ret.
-  Qed.
-
-  Lemma Returns_legacyRet_inv {E A} : forall a (t: itree E A) u,
-      t ≅ Tau u -> Returns_legacy a t -> Returns_legacy a u.
-  Proof.
-    intros * Cong Ret.
-    revert u Cong.
-    induction Ret;
-      intros.
-    - rewrite H in Cong.
-      inv_eqitree Cong.
-    - rewrite H in Cong.
-      rewrite eqitree_Tau in Cong.
-      now rewrite <- Cong.
-    - rewrite H in Cong.
-      inv_eqitree Cong.
-  Qed.
-
-  Lemma Returns_legacyVis_inv {E X A} : forall (a: A) (e: E X) k t,
-      t ≅ Vis e k -> Returns_legacy a t -> (exists x, Returns_legacy a (k x)).
-  Proof.
-    intros * Cong Ret.
-    revert X e k Cong.
-    induction Ret;
-      intros.
-    - rewrite H in Cong.
-      inv_eqitree Cong.
-    - rewrite H in Cong.
-      inv_eqitree Cong.
-    - rewrite H in Cong.
-      apply eqitree_inv_Vis_Type in Cong as EE; subst.
-      apply eqitree_inv_event in Cong as Eqee; subst.
-      exists x.
-      eapply eqit_inv_Vis in Cong.
-      now rewrite Cong in Ret.
+      intros;
+      [ apply Returns_legacyRet | apply Returns_legacyVis with X e x k];
+      case_eq b;
+      intro;
+      subst;
+      now rewrite Eq || assumption.
   Qed.
 
   Inductive Returns {A: Type} (a: A) : ccsT A -> Prop :=
